coq/theories/automation/Ltac2Utils.v
@@ -1,0 +1,196 @@
+From Ltac2 Require Import Ltac2 Std List Constr RedFlags Message.
+Import Ltac2.Constr.Unsafe.
+From Coq Require Import derive.Derive.
+From Coq Require Import Recdef.
+
+From coqutil Require Import
+  Tactics.reference_to_string
+  Tactics.ident_of_string
+  Tactics.ident_to_string.
+
+From impboot Require Import utils.Core.
+From impboot Require Import AutomationLemmas.
+
+Open Scope nat.
+
+Ltac2 opt_to_list (o: 'a option): 'a list := match o with | Some x => [x] | None => [] end.
+
+Ltac2 kind_of_constr (c: constr): string :=
+  match Unsafe.kind c with
+  | Rel _ => "Rel"
+  | Var _ => "Var"
+  | Meta _ => "Meta"
+  | Evar _ _ => "Evar"
+  | Sort _ => "Sort"
+  | Cast _ _ _ => "Cast"
+  | Prod _ _ => "Prod"
+  | Lambda _ _ => "Lambda"
+  | LetIn _ _ _ => "LetIn"
+  | App _ _ => "App"
+  | Constant _ _ => "Constant"
+  | Ind _ _ => "Ind"
+  | Constructor _ _ => "Constructor"
+  | Case _ _ _ _ _ => "Case"
+  | Fix _ _ _ _ => "Fix"
+  | CoFix _ _ _ => "CoFix"
+  | Proj _ _ _ => "Proj"
+  | Uint63 _ => "Uint63"
+  | Float _ => "Float"
+  | String _ => "String"
+  | Array _ _ _ _ => "Array"
+  end.
+
+Ltac2 reference_of_constr_opt (c: constr): reference option :=
+  match kind c with
+  | Var id => Some (Std.VarRef id)
+  | Constant const _inst => Some (Std.ConstRef const)
+  | Ind ind _inst => Some (Std.IndRef ind)
+  | Constructor cnstr _inst => Some (Std.ConstructRef cnstr)
+  | _ => None
+end.
+
+Ltac2 reference_to_string (r : reference) : string option :=
+  Some (Ident.to_string (List.last (Env.path r))).
+
+Ltac2 ident_of_fqn (fqn: string list): ident list :=
+  List.map (fun s => Option.get (Ident.of_string s)) fqn.
+
+Ltac2 messsage_of_option (o : message option) : message :=
+  match o with
+  | Some x => x
+  | None => Message.of_string "None"
+  end.
+
+Ltac2 message_of_list (l : message list) : message :=
+  let rec of_list_go (l : message list) :=
+    match l with
+    | [] => Message.of_string ""
+    | [x] => x
+    | x :: xs => Message.concat x (Message.concat (Message.of_string ",") (of_list_go xs))
+    end
+  in Message.concat (Message.of_string "[ ") (Message.concat (of_list_go l) (Message.of_string " ]")).
+
+Ltac2 messsage_of_option_constr (o : constr option) : message :=
+  match o with
+  | Some c => Message.of_constr c
+  | None => Message.of_string "None"
+  end.
+
+Ltac rewrite_let :=
+  match goal with
+  | [ |- context C [?subterm] ] =>
+    match subterm with
+    | let x := ?a in @?b x =>
+      let C' := context C [b a] in
+      change C'
+    end
+  end.
+
+Ltac unfold_fix fn :=
+  let H := fresh "H" in
+  let f := fresh "f" in
+  instantiate (1 := forall x, fn x = ?[f] x);
+  (
+    unfold fn;
+    instantiate
+      (f :=
+        ltac:(
+          let ll := fresh "ll" in
+          intros ll;
+          let thm := constr:(analyze ll) in
+          apply thm; intros
+        )
+      );
+    cbv beta;
+    match goal with
+    | [ |- forall l, _ ] =>
+        let ll := fresh l in
+        intros ll; destruct ll
+    end; fold fn; simpl analyze; reflexivity
+  );
+  cbv beta;
+  simpl analyze.
+
+Ltac unfold_tpe fn :=
+  let unfolded := ltac:(unfold_fix constr:(fn)) in
+  let t := type of ltac:(unfolded) in
+  refine t.
+
+Ltac unfold_proof :=
+  let ll := fresh "ll" in
+  intros ll;
+  cbv beta;
+  destruct ll;
+  simpl;
+  reflexivity.
+
+Ltac2 isFix (fconstr: constr): bool :=
+  let fref := reference_of_constr fconstr in
+  let unfolded := Std.eval_unfold [(fref, AllOccurrences)] fconstr in
+  Constr.is_fix unfolded.
+
+Ltac2 Type exn ::= [
+  Oopsie (string)
+].
+
+Ltac2 unfold_once (fconstr: constr) (exprconstr: constr): constr :=
+  if isFix fconstr then
+    let fref: reference option := reference_of_constr_opt fconstr in
+    let f_str: string option := Option.bind fref reference_to_string in
+    let f_equation_str: string option := Option.map (fun n => String.app n "_equation") f_str in
+    let f_equation_ident: ident list option := Option.map (fun s => ident_of_fqn [s]) f_equation_str in
+    (* print (messsage_of_option (Option.map (fun l => messsage_of_list (List.map Message.of_ident l)) f_equation_ident)); *)
+    let f_equation_ref: reference list := List.flat_map (fun id => Env.expand id) (opt_to_list f_equation_ident) in
+    match f_equation_ref with
+    | [ref] =>
+      (* TODO(kπ) should be rewrite *)
+      (* can we rewrite in constr? *)
+      Std.eval_unfold [(ref, AllOccurrences)] exprconstr
+    | _ =>
+      (* TODO(kπ) Add fconstr name or sth *)
+      Control.throw (Oopsie "No (or too many) _equation lemma found");
+      fconstr
+    end
+  else
+    let f_name_r := reference_of_constr fconstr in
+    let expr_norm := Std.eval_unfold [(f_name_r, AllOccurrences)] exprconstr in
+    expr_norm.
+
+(* Definition has_match (l: list nat) : nat :=
+  1 +
+  match l with
+  | nil => 0
+  | cons h t => h + 100
+  end.
+
+Lemma has_match_equation : ltac:(unfold_tpe has_match).
+Proof. ltac1:(unfold_proof). Qed.
+
+About has_match_equation.
+
+Fixpoint sum_n (n : nat) : nat :=
+  match n with
+  | 0 => 1 + 1
+  | S n1 => (sum_n n1)(*  + n *)
+  end.
+
+Lemma sum_n_equation : ltac:(unfold_tpe sum_n).
+Proof. ltac1:(unfold_proof). Qed.
+
+About sum_n_equation.
+
+Goal forall n, sum_n n = 1.
+Proof.
+  intros.
+  (* unfold_once constr:(sum_n) constr:(forall n, sum_n n = 1). *)
+  rewrite sum_n_equation.
+  (* ltac1:(unfold_fix sum_n). *)
+Abort.
+
+Goal forall l, has_match l = 1.
+Proof.
+  intros.
+  rewrite has_match_equation.
+  unfolded_def constr:(has_match).
+  (* ltac1:(unfold_fix has_match). *)
+Abort. *)
